WIP; behavioral equivalence

Equiv.v
@@ -1,3 +1,245 @@
 Require Export Imp.
 
+(* equivalence of expressions *)
+
+Definition aequiv (a1 a2 : aexp) : Prop :=
+    forall (st : state),
+        aeval st a1 = aeval st a2.
+
+Definition bequiv (b1 b2 : bexp) : Prop :=
+    forall (st : state),
+        beval st b1 = beval st b2.
+
+(* equivalence of programs *)
+
+Definition cequiv (c1 c2 : com) : Prop :=
+    forall (st st' : state),
+        (c1 / st || st') <-> (c2 / st || st').
+
+Theorem aequiv_example:
+    aequiv (AMinus (AId X) (AId X)) (ANum 0).
+Proof.
+    unfold aequiv. intros. simpl. omega.
+Qed.
+
+Theorem bequiv_example:
+    bequiv (BEq (AMinus (AId X) (AId X)) (ANum 0)) BTrue.
+Proof.
+    unfold bequiv. intros. simpl.
+    assert (st X - st X = 0). omega.
+    rewrite -> H. reflexivity.
+Qed.
+
+Theorem skip_left: forall c,
+    cequiv (SKIP;; c) c.
+Proof.
+    unfold cequiv. intros c st st'. split.
+    Case "->".
+        intro H. inversion H. subst.
+        inversion H2. subst. assumption.
+    Case "<-".
+        intro H. apply E_Seq with st.
+        apply E_Skip. apply H.
+Qed.
+
+Theorem skip_right: forall c,
+    cequiv (c;; SKIP) c.
+Proof.
+    unfold cequiv. intros c st st'. split.
+    Case "->".
+        intro H. inversion H. subst.
+        inversion H5. subst. assumption.
+    Case "<-".
+        intro H. apply E_Seq with st'.
+        apply H. apply E_Skip.
+Qed.
+
+Theorem IFB_true_simple: forall c1 c2,
+    cequiv (IFB BTrue THEN c1 ELSE c2 FI) c1.
+Proof.
+    unfold cequiv. intros c1 c2 st st'. split.
+    Case "->".
+        intro H. inversion H. 
+        subst. assumption.
+        subst. inversion H5.
+    Case "<-".
+        intro H. apply E_IfTrue.
+        simpl. reflexivity.
+        assumption.
+Qed.
+
+Theorem IFB_true: forall b c1 c2,
+    bequiv b BTrue ->
+    cequiv (IFB b THEN c1 ELSE c2 FI) c1.
+Proof.
+    intros b c1 c2 HbEqBtrue. unfold cequiv. split.
+    Case "->".
+        intro H. inversion H. 
+            subst. assumption.
+            subst. unfold bequiv in HbEqBtrue.
+            rewrite -> HbEqBtrue in H5. inversion H5.
+    Case "<-".
+        intro H. apply E_IfTrue.
+            unfold bequiv in HbEqBtrue.
+            rewrite -> HbEqBtrue. simpl. reflexivity.
+            assumption.            
+Qed.
+
+Theorem IFB_false: forall b c1 c2,
+    bequiv b BFalse ->
+    cequiv (IFB b THEN c1 ELSE c2 FI) c2.
+Proof.
+    intros b c1 c2 HbEqF. split; intros H.
+    Case "->".
+        inversion H; subst; try assumption.
+            (* contradictive subgoal *)
+            rewrite HbEqF in H5; inversion H5.
+    Case "<-".
+        apply E_IfFalse; try assumption.
+            (* just rewrite to finish *)
+            rewrite HbEqF; reflexivity.
+Qed.
+
+Theorem swap_if_branches: forall b e1 e2,
+    cequiv
+      (IFB b THEN e1 ELSE e2 FI)
+      (IFB BNot b THEN e2 ELSE e1 FI).
+Proof.
+    intros b e1 e2. split; intro H.
+    Case "->".
+        inversion H; subst.
+          apply E_IfFalse; try assumption.
+             simpl. rewrite -> H5. reflexivity.
+          apply E_IfTrue; try assumption.
+             simpl. rewrite -> H5. reflexivity.
+    Case "<-".
+        inversion H; subst.
+          apply E_IfFalse; try assumption.
+             simpl in H5.
+             rewrite -> negb_true_iff in H5. assumption. 
+          apply E_IfTrue; try assumption.
+             simpl in H5.
+             rewrite -> negb_false_iff in H5. assumption.
+Qed.
+
+Theorem WHILE_false: forall b c,
+    bequiv b BFalse ->
+    cequiv (WHILE b DO c END) SKIP.
+Proof.
+    intros b c Hb. split; intro H.
+    Case "->".
+        inversion H; subst.
+        SCase "E_WhileEnd".
+            apply E_Skip.
+        SCase "E_WhileLoop".
+            unfold bequiv in Hb. rewrite Hb in H2. inversion H2.
+    Case "<-".
+        inversion H; subst.
+        apply E_WhileEnd. unfold bequiv in Hb. rewrite -> Hb.
+        simpl. reflexivity.
+Qed.
+
+Lemma WHILE_true_nonterm: forall b c st st',
+    bequiv b BTrue ->
+    ~( (WHILE b DO c END) / st || st' ).
+Proof.
+    intros b c st st' Hb.
+    intro H.
+    remember (WHILE b DO c END) as cw eqn:Heqcw.
+    ceval_cases (induction H) Case;
+    (* most cases don't apply and can be clear out be inversion *)
+        inversion Heqcw; subst; clear Heqcw.
+    Case "E_WhileEnd".
+        unfold bequiv in Hb. rewrite Hb in H. inversion H.
+    Case "E_WhileLoop".
+        apply IHceval2. reflexivity. 
+Qed.
+
+Theorem WHILE_true: forall b c,
+    bequiv b BTrue ->
+    cequiv
+        (WHILE b DO c END)
+        (WHILE BTrue DO SKIP END).
+Proof.
+    intros b c Hb. split; intro H.
+    Case "->".
+       (* in the Hb context, H cannot be true, ~H actually is *)
+       assert (~(WHILE b DO c END) / st || st').
+       SCase "Proof of assert".
+           apply WHILE_true_nonterm.
+           unfold bequiv. assumption.
+       apply H0 in H. inversion H.
+    Case "<-".
+        (* H is obviously not true, but ~H is *)
+        assert (~(WHILE BTrue DO SKIP END) / st || st').
+        SCase "Proof of assert".
+            apply WHILE_true_nonterm. unfold bequiv. reflexivity.
+        apply H0 in H. inversion H.
+Qed.
+
+Theorem loop_unrolling: forall b c,
+    cequiv
+        (WHILE b DO c END)
+        (IFB b THEN (c;; WHILE b DO c END) ELSE SKIP FI).
+Proof.
+    intros b c. split; intro Hce.
+    Case "->".
+        inversion Hce; subst.
+        SCase "E_WhileEnd". apply E_IfFalse.
+            assumption.
+            apply E_Skip.
+        SCase "E_WhileLoop". apply E_IfTrue.
+            assumption.
+            apply E_Seq with st'0. assumption. assumption.
+    Case "<-".
+        inversion Hce; subst.
+        SCase "b is true, ie loop runs". inversion H5; subst.
+            apply E_WhileLoop with st'0. assumption. assumption.
+            assumption.
+        SCase "b is false, in loop ends". inversion H5; subst.
+            apply E_WhileEnd. assumption.
+Qed.
+
+Theorem seq_assoc: forall c1 c2 c3,
+    cequiv ((c1;;c2);;c3) (c1;;(c2;;c3)).
+Proof.
+    intros c1 c2 c3. split; intro H.
+    Case "->".
+        inversion H; subst. inversion H2; subst.
+        apply E_Seq with st'1.
+          assumption.
+          apply E_Seq with st'0. assumption. assumption.
+    Case "<-".
+        inversion H; subst. inversion H5; subst.
+        apply E_Seq with st'1.
+          apply E_Seq with st'0. assumption. assumption.
+          assumption.
+Qed.
+
+Axiom functional_extensionality:
+    forall {X Y : Type} {f g : X -> Y},
+    (forall (x:X), f x = g x) -> f = g.
+
+Theorem identity_assignment: forall (X:id),
+    cequiv (X ::= AId X) SKIP.
+Proof.
+    intros. split; intro H.
+    Case "->".
+        inversion H; subst. simpl. simpl in H.
+        replace (update st X (st X)) with st. constructor.
+        apply functional_extensionality.
+        intro x.
+        Check update_same.
+        rewrite -> update_same. reflexivity. reflexivity.
+    Case "<-".
+        inversion H; subst.
+        (* need to rewrite goal so that E_Ass can be applied *)
+        assert (st' = (update st' X (st' X))).
+        SCase "Proof of assert".
+            apply functional_extensionality. intro x.
+            rewrite -> update_same; reflexivity.
+        rewrite H0 at 2. (* rewrite the second occurence of st' *)
+        apply E_Ass. simpl. reflexivity.
+Qed.
+
 
